Started proof of become_leader;
for proof elegance, tried adding an explicit predicate that keeps track
of the important facts about configuration changes; something like the
"old_term_max" but for configs instead of terms. This almost worked,
except for some mutual recursion, which leads to later problems because
these predicates are put inside of an invariant. Might be able to get
around the issue with a few steps.

src/program_proof/reconf/ghost_proof.v
@@ -94,10 +94,87 @@ Definition committed_at_term γ term mval: iProp Σ :=
   ([∗ set] srv ∈ W, accepted_lb γ srv term mval)
 .
 
-Definition old_conf_max γ term mval : iProp Σ :=
-  □(∀ term' mval', ⌜int.nat term' < int.nat term⌝ →
-  (committed_at_term γ term' mval') -∗
-            ⌜mval_le mval' mval⌝
+Definition overlapping_quorums (config1 config2:ConfigC) :=
+  ∀ W1 W2, (config1.(is_quorum) W1) → (config2.(is_quorum) W2) → W1 ∩ W2 ≠ ∅.
+
+(* Maybe this should say
+   either the config of mval' intersects with the config of mval OR
+   every quorum in mval' contains a server that accepted something bigger than
+   mval'.
+*)
+(*
+  FIXME: should we take term'' = term here?
+  If we do, then it's not clear how to prove (old_conf_max γ term mval -∗
+  old_conf_max γ (term + 1) mval) anymore.
+  If we don't, then when we want to use old_conf_max, it's possible that term''
+  < term, in which case we would want to use old_term_max, but we can't use
+  old_term_max, because it requires old_conf_max.
+
+  There isn't a real circularity, it's just that we want to recursive invoke
+  old_conf and old_term. But, that'll result in later problems.
+ *)
+From iris.bi.lib Require Import fixpoint.
+
+Print fixpoint.
+
+Definition old_conf_max_pre (Φ:(reconf_names -d> u64 -d> (list (leibnizO LogEntry)) -d> iPropO Σ)): (reconf_names -d> u64 -d> (list (leibnizO LogEntry)) -d> iPropO Σ) :=
+  λ γ term mval,
+    (∀ mval', ⌜mval_lt mval' mval⌝ → □(
+        (⌜overlapping_quorums (get_config mval') (get_config mval)⌝ ∨
+         (∃ mval'' term'',
+             ⌜mval_lt mval mval''⌝ ∗
+             ⌜mval_le mval'' mval'⌝ ∗
+             ⌜int.nat term'' ≤ int.nat term⌝ ∗
+             committed_at_term γ term'' mval'' ∗
+             Φ γ term mval'' ∗
+             ⌜overlapping_quorums (get_config mval') (get_config mval'')⌝
+         )
+        )
+     ))%I
+.
+
+Definition old_conf_max_pre_least γ term Φ mval: iProp Σ :=
+  ∀ mval', ⌜mval_lt mval' mval⌝ → □(
+        (⌜overlapping_quorums (get_config mval') (get_config mval)⌝ ∨
+         (∃ mval'' term'',
+             ⌜mval_lt mval mval''⌝ ∗
+             ⌜int.nat term'' ≤ int.nat term⌝ ∗
+             committed_at_term γ term'' mval'' ∗
+             Φ mval'' ∗
+             ⌜overlapping_quorums (get_config mval') (get_config mval'')⌝
+         )
+        )
+     )
+.
+
+
+Definition old_conf_max γ term mval : iProp Σ := (bi_least_fixpoint (old_conf_max_pre_least γ term) mval).
+
+Instance old_conf_max_pre_contr : Contractive old_conf_max_pre.
+Admitted.
+
+Program Definition old_conf_max_2 γ term mval : iProp Σ := □ (fixpoint (old_conf_max_pre) γ term mval).
+
+Definition old_conf_max_orig γ term mval: iProp Σ :=
+  ∀ mval', ⌜mval_lt mval' mval⌝ → □(
+        (⌜overlapping_quorums (get_config mval') (get_config mval)⌝ ∨
+         (∃ mval'' term'',
+             ⌜mval_lt mval mval''⌝ ∗
+             ⌜int.nat term'' ≤ int.nat term⌝ ∗
+             committed_at_term γ term'' mval'' ∗
+             (* FIXME: want to be able to put another old_conf_max here *)
+             ⌜overlapping_quorums (get_config mval') (get_config mval'')⌝
+         )
+        )
+     )
+.
+
+Definition old_term_max γ term mval : iProp Σ :=
+  ∀ term' mval', □(⌜int.nat term' < int.nat term⌝ →
+  proposed_lb γ term' mval' -∗
+  committed_at_term γ term' mval' -∗
+  old_conf_max γ term' mval' -∗
+  ⌜mval_le mval' mval⌝
   )
 .
 
@@ -109,13 +186,11 @@ Definition sys_inv γ : iProp Σ :=
           commit γ mval ∗
           (committed_at_term γ term mval) ∗
           proposed_lb γ term mval ∗
-          old_conf_max γ term mval (* XXX: could make a accepted_lb_fancy, and put this
+          old_term_max γ term mval ∗ (* XXX: could make a accepted_lb_fancy, and put this
                               in there, and add requirement that quorum is
                               non-empty. *)
+          old_conf_max γ term mval
   ).
-
-Definition overlapping_quorums (config1 config2:ConfigC) :=
-  ∀ W1 W2, (config1.(is_quorum) W1) → (config2.(is_quorum) W2) → W1 ∩ W2 ≠ ∅.
 
 Definition no_concurrent_reconfigs_and_overlapping_quorums γ term mval : iProp Σ :=
   ∃ mval',
@@ -145,33 +220,68 @@ Proof.
   apply (transitivity H1 H0).
 Qed.
 
+Instance test γ term: BiMonoPred (old_conf_max_pre_least γ term).
+Proof.
+  apply Build_BiMonoPred.
+  {
+    iIntros (????) "#Hwand".
+    iIntros (?) "#H".
+    iIntros (??) "!#".
+    iSpecialize ("H" $! mval' H1 with "").
+    iDestruct "H" as "[H|H]".
+    {
+      iLeft.
+      done.
+    }
+    {
+      iRight.
+      iDestruct "H" as (??) "H".
+      iExists _, _; iFrame "#".
+      admit.
+    }
+  }
+  {
+    admit.
+  }
+Admitted.
+
 Lemma ghost_commit γ term mval :
   sys_inv γ -∗
   committed_at_term γ term mval -∗
   proposed_lb γ term mval -∗
-  old_conf_max γ term mval (* XXX: could make a accepted_lb_fancy, and put this
+  old_term_max γ term mval -∗ (* XXX: could make a accepted_lb_fancy, and put this
                               in there, and add requirement that quorum is
                               non-empty. *)
+  old_conf_max γ term mval
   ={↑sysN}=∗
   commit_lb γ mval
 .
 Proof.
-  iIntros "#Hinv #HcommitAt #Hproposed #Hold".
-  iInv "Hinv" as ">Hi" "Hclose".
-  iDestruct "Hi" as (commitTerm commitVal) "(Hcommit & #HcommitAcc & #HproposedCommit & #HoldCommit)".
+  iIntros "#Hinv #HcommitAt #Hproposed #Hold Hconf".
+  unfold old_conf_max.
+  rewrite least_fixpoint_unfold.
+  iDestruct "Hconf" as "#Hconf".
+  iInv "Hinv" as "Hi" "Hclose".
+  iDestruct "Hi" as (commitTerm commitVal) "Hi".
+  iEval (unfold old_conf_max) in "Hi".
+  rewrite least_fixpoint_unfold.
+  iDestruct "Hi" as "(>Hcommit & #>HcommitAcc & #>HproposedCommit & #>HoldCommit & #HconfCommit)".
   iAssert (⌜mval_le mval commitVal ∨ mval_le commitVal mval⌝)%I as "%Hcomparable".
   {
     destruct (decide (int.nat term < int.nat commitTerm)).
     { (* case: term < commitTerm *)
-      iDestruct ("HoldCommit" with "[] HcommitAt") as "%HvalLe".
+      iDestruct ("HoldCommit" with "[] Hproposed HcommitAt [Hconf]") as "%HvalLe".
       { done. }
+      {
+        unfold old_conf_max.
+        rewrite least_fixpoint_unfold.
+        iFrame "Hconf".
+      }
       eauto.
     }
     destruct (decide (int.nat term = int.nat commitTerm)).
     { (* case: term == commitTerm *)
       replace (commitTerm) with (term) by word.
-      (* TODO: put together the proposed_lb's to know that one of them is bigger
-       than the other. *)
       iDestruct (own_valid_2 with "Hproposed HproposedCommit") as %Hvalid.
       rewrite singleton_op in Hvalid.
       apply singleton_valid in Hvalid.
@@ -180,8 +290,14 @@ Proof.
     }
     (* case: term > commitTerm *)
     assert (int.nat term > int.nat commitTerm) by word.
-    iDestruct ("Hold" with "[] HcommitAcc") as "%HvalLe".
+    iDestruct ("Hold" with "[] HproposedCommit HcommitAcc [HconfCommit]") as "%HvalLe".
     { done. }
+    {
+      iIntros.
+      unfold old_conf_max.
+      rewrite least_fixpoint_unfold.
+      iFrame "HconfCommit".
+    }
     eauto.
   }
 
@@ -215,7 +331,7 @@ Proof.
     {
       iNext.
       iExists _, _; iFrame.
-      iFrame "#".
+      iFrame "HcommitAt #".
     }
     done.
   }
@@ -227,13 +343,96 @@ Lemma become_leader γ term highestVal :
     (get_config highestVal).(is_quorum) W →
     sys_inv γ -∗
     proposed_lb_fancy γ highestTerm highestVal -∗
+    old_term_max γ highestTerm highestVal -∗
+    old_conf_max γ highestTerm highestVal -∗
     □(
       [∗ set] srv ∈ W,
         (∃ srvVal, ⌜mval_le srvVal highestVal⌝ ∗ accepted_ro γ srv highestTerm srvVal) ∗
         (∀ term', ⌜int.nat highestTerm < int.nat term'⌝ → ⌜int.nat term' < int.nat term⌝ → accepted_ro_none γ srv term')
-    ) ={↑sysN}=∗
-    old_conf_max γ term highestVal.
+    ) -∗
+    old_term_max γ term highestVal.
 Proof.
-Admitted.
+  intros ? ? HtermIneq Hquorum.
+  iIntros "#Hsys #Hproposed #Hold #Hconf #HoldInfo".
+  iIntros (term' mval').
+  iModIntro.
+  iIntros "%Hterm'Ineq".
+  iIntros "#Hproposed'".
+  iIntros "#Hcommit' #Hconf'".
+  destruct (decide (int.nat term' < int.nat highestTerm)).
+  { (* term' < highestTerm, so we can just use the old_term_max of (highestTerm,highestVal) *)
+    by iApply "Hold".
+  }
+  destruct (decide (int.nat term' = int.nat highestTerm)).
+  { (* for term' == highestTerm, we have the first part of "oldInfo" *)
+    replace (term') with (highestTerm); last first.
+    { (* FIXME: why doesn't word work? *)
+      clear -e.
+      Search Z.to_nat.
+      rewrite Z2Nat.inj_iff in e; first last.
+      { word. }
+      { word. }
+      {
+        Search word.unsigned.
+        apply word.unsigned_inj in e.
+        done.
+      }
+    }
+    iDestruct "Hproposed" as "[Hproposed Hfancy]".
+    iDestruct (own_valid_2 with "Hproposed' Hproposed") as %Hvalid.
+    rewrite singleton_op in Hvalid.
+    rewrite singleton_valid in Hvalid.
+    apply mono_list_lb_op_valid_1_L in Hvalid.
+    destruct Hvalid as [Hdone|HlogLe].
+    { done. }
+    destruct (decide (length mval' = length highestVal)).
+    { (* If the two are equal, then no problem *)
+      assert (mval' = highestVal).
+      {
+        symmetry.
+        apply list_prefix_eq.
+        {
+          done.
+        }
+        word.
+      }
+      rewrite H.
+      done.
+    }
+    (* case: mval_lt highestVal mval'. Here, we're gonna derive a contradiction. *)
+    iExFalso.
+    (* now, apply old_conf_max highestTerm mval'' *)
+    iDestruct ("Hconf'" $! highestVal) as "#Hconf2".
+    iSpecialize ("Hconf2" with "[]").
+    {
+      iPureIntro.
+      split; naive_solver.
+    }
+    iDestruct "Hconf2" as "[Hoverlap|Hstale]".
+    { (* In this case, the quorums of mval' overlap with the quorums of highestVal.
+         This gives a contradiction between Hcommit' and HoldInfo.
+       *)
+      admit.
+    }
+    { (* In this case, some highest value mval'' was committed, and has
+         overlapping quorums with highestVal. *)
+      iDestruct "Hstale" as (mval'' term'') "(%Hmval''lt & %Hterm''Ineq & Hcommit'' & %Hoverlap)".
+      (* if term'' < highestTerm, then (old_term_max highestTerm highestVal) takes care of it *)
+      destruct (decide (int.nat term'' < int.nat highestTerm)).
+      {
+        iSpecialize ("Hold" $! term'' mval'' with "[] [] Hcommit''").
+        { done. }
+        {  admit. } (* TODO: add this to old_conf_max. *)
+        (* FIXME: we need old_conf_max to finish instantiating the old_term_max.
+           But, we need old_conf_max for the term'' and mval'' that we
+           destructed from a different old_conf_max.
+         *)
+      }
+      assert (term'' = highestTerm) as -> by word.
+      admit. (* TODO: need to know that mval'' > highestVal to get contradiction *)
+    }
+
+  }
+
 
 End ghost_proof.
